

23/28

IFT-6155 Quantum Computing

---

**Assignment 2**

---

*Ayoub Echchahed*

*Nassim El Massaudi*

Presented to  
Mr. Gilles Brassard

Department of Computer Science and Operations Research  
University of Montreal  
Winter 2023

### Question 1

- Find a transformation  $S$  whose composition with itself provides true logical negation.
- In other words, it must be that  $S^2 = X$ , which means that  $S^2|\Psi\rangle = X|\Psi\rangle$  for all  $|\Psi\rangle$

5/5

- Steps:
- 1) Decomposition of the transformation
  - 2) Computations for finding the eigenvalues
  - 3) Computations for finding the eigenvectors
  - 4) Finding  $Q^{-1}$  from  $Q$
  - 5) Determining  $S$
  - 6) Demonstrating  $S^2 = X$

Question 1:

Find  $S$  such as  $S^2 = X$ ,  $S \in M_2(\mathbb{C})$

$X = \begin{bmatrix} 0 & 1 \\ 1 & 0 \end{bmatrix}$

Let  $|\Psi\rangle = \begin{bmatrix} x \\ y \end{bmatrix}$ .

We can decompose  $X$  as follow:

$X = S^2 = Q \Lambda Q^{-1}$ , where  $\Lambda = \begin{bmatrix} \lambda_1 & 0 \\ 0 & \lambda_2 \end{bmatrix}$ .

Let's calculate the eigenvalues and eigenvectors of  $X$ .

Let's resolve  $X - \lambda I_2 = 0$ .

$X - \lambda I_2 = \begin{bmatrix} 0 & 1 \\ 1 & 0 \end{bmatrix} - \begin{bmatrix} \lambda & 0 \\ 0 & \lambda \end{bmatrix} = \begin{bmatrix} -\lambda & 1 \\ 1 & -\lambda \end{bmatrix} = 0$ .

$\Rightarrow \det(X - \lambda I_2) = \lambda^2 - 1 = (\lambda - 1)(\lambda + 1) = 0$ .

The roots are  $\lambda_1 = 1, \lambda_2 = -1$ .

Next, let's find the eigenvectors.

-  $\lambda = 1$ , the reduced row echelon is  $\begin{bmatrix} 0 & 1 \\ 0 & 0 \end{bmatrix}$ .

Let's find its null space,

$\begin{bmatrix} 0 & 1 \\ 0 & 0 \end{bmatrix} \begin{bmatrix} x \\ y \end{bmatrix} = \begin{bmatrix} 0 \\ 0 \end{bmatrix} \Leftrightarrow \vec{x} = \begin{bmatrix} 1 \\ 0 \end{bmatrix} t$ .

So, the eigenvector  $\vec{x}_1 = \begin{bmatrix} 1 \\ 0 \end{bmatrix}$ .

Question 1: part 2

$\lambda_2 = -1$ , the reduced row echelon is  $\begin{bmatrix} 1 & 0 \\ 0 & 0 \end{bmatrix}$

To find the null space,

$\begin{bmatrix} 1 & 0 \\ 0 & 0 \end{bmatrix} \vec{x} = \begin{bmatrix} 0 \\ 0 \end{bmatrix} \Leftrightarrow \vec{x} = \begin{bmatrix} 0 \\ 1 \end{bmatrix} t, t \in \mathbb{R}^2$ .

Thus, the eigenvector is  $\vec{x}_2 = \begin{bmatrix} 0 \\ 1 \end{bmatrix}$ .

Then, let's determine  $Q^{-1}$ .

$Q = \begin{bmatrix} 1 & -1 \\ 1 & 1 \end{bmatrix} \Rightarrow Q^{-1} = \frac{1}{\det Q} \text{adj } Q = \frac{1}{2} \begin{bmatrix} 1 & 1 \\ -1 & 1 \end{bmatrix}$

Thus, we have:

$X = S^2 = Q \Lambda Q^{-1} = \begin{bmatrix} 1 & -1 \\ 1 & 1 \end{bmatrix} \begin{bmatrix} 1 & 0 \\ 0 & -1 \end{bmatrix} \begin{bmatrix} 1/2 & 1/2 \\ -1/2 & 1/2 \end{bmatrix}$

Then,  $S = Q \Lambda^{1/2} Q^{-1} = \begin{bmatrix} 1 & -1 \\ 1 & 1 \end{bmatrix} \begin{bmatrix} 1 & 0 \\ 0 & i \end{bmatrix} \begin{bmatrix} 1/2 & 1/2 \\ -1/2 & 1/2 \end{bmatrix}$

$S = \frac{1}{2} \begin{bmatrix} 1+i & 1-i \\ 1-i & 1+i \end{bmatrix}$ .

$S|\Psi\rangle = \frac{1}{2} \begin{bmatrix} 1+i & 1-i \\ 1-i & 1+i \end{bmatrix} \begin{pmatrix} \alpha \\ \beta \end{pmatrix} = \frac{1}{2} \begin{pmatrix} \alpha(1+i) + \beta(1-i) \\ \alpha(1-i) + \beta(1+i) \end{pmatrix}$

$\Rightarrow S^2|\Psi\rangle = \frac{1}{2} \begin{bmatrix} 1+i & 1-i \\ 1-i & 1+i \end{bmatrix} \frac{1}{2} \begin{pmatrix} \alpha(1+i) + \beta(1-i) \\ \alpha(1-i) + \beta(1+i) \end{pmatrix}$

$= \frac{1}{4} \begin{pmatrix} \alpha(1+i)^2 + \beta(1-i)^2 + \alpha(1-i)^2 + \beta(1+i)^2 \\ \alpha(1+i)(1-i) + \beta(1-i)(1+i) + \alpha(1-i)(1+i) + \beta(1+i)(1-i) \end{pmatrix}$

$= \frac{1}{4} \begin{pmatrix} 4\alpha & 4\beta \\ 4\alpha & 4\beta \end{pmatrix} = \begin{pmatrix} \alpha & \beta \\ \alpha & \beta \end{pmatrix} = \begin{pmatrix} \alpha \\ \beta \end{pmatrix} = \text{CPT}$



## Question 2

- **abcd Theorem:** Prove that any two-qubit state  $|\Gamma\rangle$  as given in Equation 2.10 is separable if and only if  $ad = bc$ .

- The "only if" part has already been established above; no need to repeat the argument. For the "if" part, exhibit explicit values for complex numbers  $\alpha, \beta, \gamma$  and  $\delta$  (as functions of  $a, b, c$  and  $d$ ) such that if we define one-qubit states  $|\Psi\rangle = \alpha|0\rangle + \beta|1\rangle$  and  $|\Phi\rangle = \gamma|0\rangle + \delta|1\rangle$ , then  $|\Gamma\rangle = |\Psi\rangle \otimes |\Phi\rangle$ .

$$|\Gamma\rangle = a|00\rangle + b|01\rangle + c|10\rangle + d|11\rangle \quad (2.10)$$

- Of course, both  $|\Psi\rangle$  and  $|\Phi\rangle$  must be legitimate states, meaning that  $|\alpha|^2 + |\beta|^2 = 1$  and  $|\gamma|^2 + |\delta|^2 = 1$ .

- Note that if either one of  $|\Psi\rangle$  or  $|\Phi\rangle$  is proven to be normalized, then the normalization of the other follows from the fact that  $|\Gamma\rangle = |\Psi\rangle \otimes |\Phi\rangle$  and of course that  $|\Gamma\rangle$  itself is normalized since it is given as a quantum state.

- Hint: To prove the "if" part, you may need to consider as a special (easy) case the situation in which  $abcd = 0$ , which means that at least one of  $a$  or  $d$  and at least one of  $b$  or  $c$  equals 0 since  $ad = bc$ .

Question 2: ( $ad = bc = 0 \Rightarrow$  separable).

Let's consider  $|\Psi\rangle = a|00\rangle + b|01\rangle + c|10\rangle + d|11\rangle$  such that  $ad = bc = 0$ . Note that  $\|\Psi\|^2 = |a|^2 + |b|^2 + |c|^2 + |d|^2 = 1$  which means that  $|\Psi\rangle$  is normalized.

wlog, let's assume at least one of  $a, b, c, d \in \mathbb{C}$  is not null.

So, let's assume  $a \neq 0$ , and thus,  $d = \frac{bc}{a}$ .

By definition ( $\Psi$  is separable), we can assume that  $\exists v, w \in K$  such as

$$|\Psi\rangle = |v\rangle \otimes |w\rangle = (a|0\rangle + c|1\rangle) \otimes (|0\rangle + \frac{b}{a}|1\rangle) = a|00\rangle + b|01\rangle + c|10\rangle + \frac{bc}{a}|11\rangle.$$

In this decomposition, we have  $\|w\|^2 = 1 + |\frac{b}{a}|^2 > 1$ . So  $|w\rangle$  is not normalized, let's consider  $\lambda \in \mathbb{R}_+^*$  such that:

$$\lambda = \frac{1}{\|w\|} = \frac{1}{\sqrt{|a|^2 + |c|^2}}, \text{ thus we have, } \|\lambda w\| = 1 \text{ and } \lambda w = \frac{1}{\sqrt{|a|^2 + |c|^2}} (a|0\rangle + c|1\rangle).$$

$$\|\frac{w}{\lambda}\| = \frac{\|w\|}{\lambda} = \frac{\sqrt{|a|^2 + |c|^2}}{\frac{1}{\sqrt{|a|^2 + |c|^2}}} = |a|^2 + |c|^2 = |a|^2 + |b|^2 + |c|^2 + |\frac{bc}{a}|^2 = \|\Psi\|^2 = 1.$$

$$\text{Also, } \|\lambda w\|^2 \|\frac{w}{\lambda}\| = \|w\| \|w\| = (|a|^2 + |c|^2) (1 + |\frac{b}{a}|^2) = |a|^2 + |b|^2 + |c|^2 + |\frac{bc}{a}|^2 = |a|^2 + |b|^2 + |c|^2 + |d|^2 = \|\Psi\|^2 = 1.$$

We can conclude that  $|\Psi\rangle$  is separable if  $ad = bc$ . Q.E.D.

et si  $a=0$ ?

Ceci se t  
à rien?

Je présume qu'ici, vous voulez dire  $|\frac{w}{\lambda}|^2$ .

Ce qui serait:  $(|a|^2 + |c|^2)(1 + |b/a|^2)$

et qui n'a aucun rapport avec ce qui est écrit.

Question 3

4/5

A)

**Exercise 2.5.2** Consider an arbitrary one-qubit unitary transformation  $U$  and apply it independently to each qubit of a  $|\Psi^-\rangle$  pair. Prove that the resulting state is again  $|\Psi^-\rangle$ , possibly up to an irrelevant phase factor. In other words, prove that there exists a complex number  $\eta$  of unit norm, which depends only on  $U$ , such that

$$[U \otimes U]|\Psi^-\rangle = \frac{1}{\sqrt{2}}(U|0\rangle \otimes U|1\rangle) - \frac{1}{\sqrt{2}}(U|1\rangle \otimes U|0\rangle) = \eta|\Psi^-\rangle.$$

Give explicitly the value of  $\eta$  as a function of the parameters  $\alpha, \beta, \gamma$  and  $\delta$  so that  $U|0\rangle = \alpha|0\rangle + \beta|1\rangle$  and  $U|1\rangle = \gamma|0\rangle + \delta|1\rangle$ .  $\square$

2.5.2 :

$$\begin{aligned} [U \otimes U]|\Psi^-\rangle &= \frac{1}{\sqrt{2}}(U|0\rangle \otimes U|1\rangle) - \frac{1}{\sqrt{2}}(U|1\rangle \otimes U|0\rangle) \\ &= \frac{1}{\sqrt{2}}[(\alpha|0\rangle + \beta|1\rangle) \otimes (\gamma|0\rangle + \delta|1\rangle) - (\gamma|0\rangle + \delta|1\rangle) \otimes (\alpha|0\rangle + \beta|1\rangle)] \\ &= \frac{1}{\sqrt{2}}[(\alpha\gamma|00\rangle + \alpha\delta|01\rangle + \beta\gamma|10\rangle + \beta\delta|11\rangle) - (\gamma\alpha|00\rangle + \gamma\beta|01\rangle + \delta\alpha|10\rangle + \delta\beta|11\rangle)] \\ &= \frac{1}{\sqrt{2}}[(\beta\gamma - \delta\alpha)|10\rangle + (\alpha\delta - \gamma\beta)|01\rangle] \\ &= \frac{\alpha\delta - \gamma\beta}{\sqrt{2}}|01\rangle - \frac{\delta\alpha - \beta\gamma}{\sqrt{2}}|10\rangle = (\delta\alpha - \beta\gamma)|\Psi^-\rangle. \end{aligned}$$

On a donc  $\eta = (\delta\alpha - \beta\gamma)$  où  $\alpha, \beta, \gamma, \delta \in \mathbb{C}$ .

Est-ce que  $|\eta| = 1$ ?



B)

5/5

**Exercise 2.5.3** First prove that  $|\Phi^+\rangle$  is invariant under bilateral application of the Hadamard transform:  $[H \otimes H]|\Phi^+\rangle = |\Phi^+\rangle$ . In contrast to Exercise 2.5.2, however, find explicitly a one-qubit unitary transformation  $U$  such that  $[U \otimes U]|\Phi^+\rangle \neq |\Phi^+\rangle$ , even up to an irrelevant phase factor. (Hint: Use complex numbers in your definition of  $U$ .) Your solution must be such that if  $U$  is applied bilaterally to each qubit forming  $|\Phi^+\rangle$ , and if the resulting state is observed, two opposite bits will be obtained with certainty (this cannot be farther away from a  $|\Phi^+\rangle$ ). Optional: Generalize this result by proving that no two-qubit state  $|\Lambda\rangle$  can exist with the property that the amplitude of both  $|01\rangle$  and  $|10\rangle$  is zero in  $[U \otimes U]|\Lambda\rangle$  for every one-qubit unitary transformation  $U$ .  $\square$

2.5.3:

$$\begin{aligned} [H \otimes H]|\Phi^+\rangle &= \frac{1}{\sqrt{2}} [(H|0\rangle \otimes H|0\rangle) + (H|1\rangle \otimes H|1\rangle)] \\ &= \frac{1}{\sqrt{2}} \left[ \left( \frac{1}{\sqrt{2}}|0\rangle + \frac{1}{\sqrt{2}}|1\rangle \right) \otimes \left( \frac{1}{\sqrt{2}}|0\rangle + \frac{1}{\sqrt{2}}|1\rangle \right) + \left( \frac{1}{\sqrt{2}}|0\rangle - \frac{1}{\sqrt{2}}|1\rangle \right) \otimes \left( \frac{1}{\sqrt{2}}|0\rangle - \frac{1}{\sqrt{2}}|1\rangle \right) \right] \\ &= \frac{1}{2\sqrt{2}} [ |00\rangle + |01\rangle + |10\rangle + |11\rangle + |00\rangle - |01\rangle - |10\rangle + |11\rangle ] \\ &= \frac{1}{2\sqrt{2}} [ 2|00\rangle + 2|11\rangle ] = \frac{1}{\sqrt{2}} |00\rangle + \frac{1}{\sqrt{2}} |11\rangle = |\Phi^+\rangle. \end{aligned}$$

Proof 2.5.3.

$$\begin{aligned} (U \otimes U)|\Phi^+\rangle &= \frac{1}{\sqrt{2}} [(U|0\rangle \otimes U|0\rangle) + (U|1\rangle \otimes U|1\rangle)] \\ &= \frac{1}{\sqrt{2}} [(\alpha|0\rangle + \beta|1\rangle) \otimes (\alpha|0\rangle + \beta|1\rangle) + (\gamma|0\rangle + \delta|1\rangle) \otimes (\gamma|0\rangle + \delta|1\rangle)] \\ &= \frac{1}{\sqrt{2}} [\alpha^2|00\rangle + \alpha\beta|01\rangle + \alpha\beta|10\rangle + \beta^2|11\rangle + \gamma^2|00\rangle + \gamma\delta|01\rangle + \gamma\delta|10\rangle + \delta^2|11\rangle] \\ &= \frac{1}{\sqrt{2}} [(\alpha^2 + \gamma^2)|00\rangle + (\beta^2 + \delta^2)|11\rangle + (\alpha\beta + \gamma\delta)|01\rangle + (\alpha\beta + \gamma\delta)|10\rangle] \\ &= \frac{1}{\sqrt{2}} [(\alpha^2 + \gamma^2)|00\rangle + (\beta^2 + \delta^2)|11\rangle] + (\alpha\beta + \gamma\delta)|\Psi^+\rangle \end{aligned}$$

En prenant  $\alpha = \frac{1}{\sqrt{2}}, \beta = \frac{i}{\sqrt{2}}, \gamma = \frac{i}{\sqrt{2}}, \delta = -\frac{1}{\sqrt{2}}$

On a  $|\alpha|^2 + |\gamma|^2 = \frac{1}{2} + \frac{1}{2} = 1$

$|\beta|^2 + |\delta|^2 = \left| \frac{i}{\sqrt{2}} \right|^2 + \left| -\frac{1}{\sqrt{2}} \right|^2 = 1$

$\alpha\gamma^* + \beta\delta^* = \frac{1}{\sqrt{2}} \cdot \frac{i}{\sqrt{2}} + \frac{i}{\sqrt{2}} \cdot \frac{1}{\sqrt{2}} = 0$

$|\alpha|^2 + |\beta|^2 = 1$

$|\gamma|^2 + |\delta|^2 = 1$

$U = \begin{bmatrix} \alpha & \beta \\ \gamma & \delta \end{bmatrix} = \begin{bmatrix} 1/\sqrt{2} & i/\sqrt{2} \\ i/\sqrt{2} & -1/\sqrt{2} \end{bmatrix}$

#### Question 4

5/5

Question 4. Soit  $R_\theta$  l'opération de rotation de polarisation de photon par un angle  $\theta$  dans le sens antihoraire, qui envoie  $|0\rangle = |0^\circ\rangle$  et  $|1\rangle = |90^\circ\rangle$  sur

$$|\theta\rangle = (\cos \theta)|0\rangle + (\sin \theta)|1\rangle$$

et

$$|90^\circ + \theta\rangle = (\cos(90^\circ + \theta))|0\rangle + (\sin(90^\circ + \theta))|1\rangle = -(\sin \theta)|0\rangle + (\cos \theta)|1\rangle,$$

respectivement. En d'autres termes,

$$R_\theta : \begin{cases} |0\rangle \mapsto (\cos \theta)|0\rangle + (\sin \theta)|1\rangle \\ |1\rangle \mapsto -(\sin \theta)|0\rangle + (\cos \theta)|1\rangle. \end{cases}$$

Considérons également les quatre états suivants sur deux qubits :

$$|\Phi^+\rangle = \frac{1}{\sqrt{2}}(|00\rangle + |11\rangle) \quad |\Phi^-\rangle = \frac{1}{\sqrt{2}}(|00\rangle - |11\rangle)$$

$$|\Psi^+\rangle = \frac{1}{\sqrt{2}}(|01\rangle + |10\rangle) \quad |\Psi^-\rangle = \frac{1}{\sqrt{2}}(|01\rangle - |10\rangle).$$

qui portent le nom d'« états de Bell ».

Calculez l'effet d'une rotation par un angle  $\theta$  du premier qubit et par un angle  $\phi$  du second qubit de  $|\Phi^+\rangle$ , où  $\theta$  et  $\phi$  sont deux angles arbitraires. En d'autres termes, calculez

$$(R_\theta \otimes R_\phi) |\Phi^+\rangle.$$

Exprimez votre réponse le plus simplement possible en termes d'états de Bell.

Rappel :  $\sin(a-b) = \sin a \cos b - \cos a \sin b$ ;  $\cos(a-b) = \sin a \sin b + \cos a \cos b$ .

$$\begin{aligned} (R_\theta \otimes R_\phi) |\Phi^+\rangle &= \frac{1}{\sqrt{2}} (R_\theta |0\rangle \otimes R_\phi |0\rangle) + \frac{1}{\sqrt{2}} (R_\theta |1\rangle \otimes R_\phi |1\rangle) \\ &= \frac{1}{\sqrt{2}} \left( (\cos \theta |0\rangle + \sin \theta |1\rangle) \otimes (\cos \phi |0\rangle + \sin \phi |1\rangle) \right. \\ &\quad \left. + \frac{1}{\sqrt{2}} \left( (-\sin \theta |0\rangle + (\cos \theta |1\rangle) \otimes (-\sin \phi |0\rangle + (\cos \phi |1\rangle) \right) \right) \\ &= \frac{\cos \theta \cdot \cos \phi}{\sqrt{2}} |00\rangle + \frac{\sin \theta \cdot \sin \phi}{\sqrt{2}} |11\rangle + \frac{\cos \theta \cdot \sin \phi}{\sqrt{2}} |01\rangle \\ &\quad + \frac{\sin \theta \cdot \cos \phi}{\sqrt{2}} |10\rangle \\ &\quad + \frac{-(\sin \theta) \cdot (-\sin \phi)}{\sqrt{2}} |00\rangle + \frac{-(\sin \theta) \cdot (\cos \phi)}{\sqrt{2}} |01\rangle + \frac{\cos \theta \cdot (-\sin \phi)}{\sqrt{2}} |10\rangle \\ &\quad + \frac{(\cos \theta) \cdot (\cos \phi)}{\sqrt{2}} |11\rangle \\ &= \frac{1}{\sqrt{2}} \left( [(\cos \theta \cdot \cos \phi) + (-\sin \theta) \cdot (-\sin \phi)] |00\rangle \right. \\ &\quad + [(\cos \theta \cdot \sin \phi) + (-\sin \theta) \cdot (\cos \phi)] |01\rangle \\ &\quad + [(\sin \theta \cdot \cos \phi) + (\cos \theta \cdot (-\sin \phi))] |10\rangle \\ &\quad \left. + [(\sin \theta \cdot \sin \phi) + (\cos \theta \cdot \cos \phi)] |11\rangle \right) \\ &= \frac{1}{\sqrt{2}} (\cos(\theta - \phi) |00\rangle + \sin(\theta - \phi) |01\rangle - \sin(\theta - \phi) |10\rangle \\ &\quad + \cos(\theta - \phi) |11\rangle) \\ &= \cos(\theta - \phi) |\Phi^+\rangle + \sin(\theta - \phi) |\Psi^-\rangle. \end{aligned}$$